#матан 
# Пример
$$\frac{1}{x^3 + 1} = \frac{1}{(x + 1)(x^2 - x + 1)} = \frac{A}{x + 1} + \frac{Mx + N}{x^2 - x + 1} = $$
$$= \frac{A(x^2 - x + 1) + (x + 1)(Mx + N)}{(x + 1)(x^2 - x + 1)} = \frac{1}{x^3 + 1}$$
# Метод неопр. коэффициентов
## Способ 2:
1. $Ax^2 - Ax + A + Mx^2 + Nx + Mx + N = 1 \cdot x^0 + 0 \cdot x^1 + 0 \cdot x^2 = 1$
2. $\begin{cases} x^0: \ A + N = 1 \implies A = 1 - N \\ x^1: \ -A + N + M = 0 \implies 1 + 2N + M = 0 \\ x^2: \ A + M = 0 \implies 1 - N + M = 0\end{cases}$
3. $\begin{cases} M + 2N - 1 = 0 \\ 1 - N + M = 0\end{cases}$
4. $2N - 1 - 1 + N = 0$
5. $3N = 2 \implies N \ \frac{2}{3} \implies M = -\frac{1}{3}, \ A = \frac{1}{3}$
## Способ 1:
1. $x = -1$
2. $1 = A (x^2 - x + 1) + (Mx + N)(x + 1)$
3. $A = \frac{1}{x^2 - x + 1} = \frac{1}{3}$
4. $x = 0 \implies 1 = A + N \implies N \ \frac{2}{3}$
5. $x = 1 \implies A + (M + N) \cdot 2 = 1 \implies M = \frac{1 - A}{2}$
## Пример
- $$\int \frac{x^4}{x^3 + 1}dx = \int (x - \frac{x}{x^3 + 1})dx = \int xdx - (\int \frac{A}{(x + 1)}dx + \int \frac{Mx + N}{x^2 - x + 1}dx)$$
- $A(x^2 - x + 1) + (Mx + N)(x + 1) = x$
1. $x = -1$
	$A = \frac{x}{x^2 - x + 1} = -\frac{1}{3}$
2. $x^0: \  A + N = 0 \implies N = 0 - A = \frac{1}{3}$
3. $x^1: \  -A + M + N = 1 \implies M = 1 - N + A = 1 - \frac{1}{3} - \frac{1}{3} = \frac{1}{3}$
4. $$\frac{x^2}{2} + \int \frac{1}{3(x + 1)}dx - \frac{1}{3}\int \frac{x + 1}{x^2 - x + 1}dx = \frac{x^2}{2} + \frac{1}{3}ln|x + 1| -$$ $$- \frac{1}{3} (\int \frac{\frac{1}{2} (2x + 1)}{x^2 - x + 1}dx + \frac{3}{2}\int \frac{1}{(x - \frac{1}{2})^2 + \frac{3}{4}}dx) = $$ $$= \frac{x^2}{2} + \frac{1}{3} ln|x + 1| - \frac{1}{6} ln|x^2 - x + 1| - \frac{1}{\sqrt{3}} arctg(\frac{x - \frac{1}{2}}{\frac{\sqrt{3}}{2}}) + C$$