#матан 
## Номер 1

$f(x) = \begin{cases} -x, \ x \in [-\pi, 0] \\ x, \ \frac{x^2}{\pi} \in (0, \pi] \end{cases}, \ T = 2\pi, \ l = \pi, \ w = \frac{2 \pi}{T} = 1$

![[Pasted image 20241206094114.png|400]]

- $a_0 = \frac{1}{2 \pi} \int\limits_{l}^{l} f(x) dx = \frac{1}{2 \pi} (- \int\limits_{\pi}^{0} x dx + \int\limits_{0}{\pi} \frac{x^2}{\pi} dx) = \frac{1}{2 \pi} (- \frac{x^2}{2}|_{- \pi}^{0} + \frac{x^3}{3 \pi} |_{0}^{\pi}) = \frac{1}{2 \pi} (\frac{\pi ^ 2}{2} + \frac{\pi^3}{3 \pi}) = \frac{\pi}{4} + \frac{\pi}{6} = \frac{5 \pi}{12}$
- $a_n = \frac{1}{l} \int\limits_{-l}^{l} f(x) \cos (nwx) dx = \frac{1}{\pi} (\int\limits_{- \pi}^{0} x \cos (nx) dx + \int\limits_{0}^{\pi} \frac{x^2}{\pi} \cos (nx) dx) = (*)$
	$I = \begin{vmatrix} u = x \\ du = dx \\ dv = \cos(nx) dx \\ v = \frac{\sin (nx)}{n} \end{vmatrix} = x \frac{\sin (nx)}{n}|_{- \pi}^{0} - \int\limits_{- \pi}^{0} \frac{\sin (nx)}{n} dx = \frac{\cos (nx)}{n^2}|_{- \pi}^{0} = \frac{1}{n^2} - \frac{(-1)^n}{n^2}$
	$II = \begin{vmatrix} u = x^2 \\ du = \frac{2x}{\pi}dx \\ dv = \cos(nx) dx \\ v = \frac{\sin (nx)}{n} \end{vmatrix} = x^2 \frac{\sin(nx)}{n}|_{0}^{\pi} - \frac{2}{\pi} \int\limits_{0}^{\pi} x \frac{\sin (nx)}{n}dx = \begin{vmatrix} u = x \\ du = dx \\ dv = \frac{\sin(nx)}{n} dx \\ v = \frac{- \cos (nx)}{n^2} \end{vmatrix} = \frac{2}{\pi}(x \frac{\cos (nx)}{n^2}|_{0}^{\pi} - \int\limits_{0}^{\pi} \frac{\cos(nx)}{n^2}) = \frac{2}{\pi}x \frac{\cos (nx)}{n^2}|_{0}^{\pi} - \frac{2}{\pi} \frac{\sin (nx)}{n^3}|_{0}^{\pi} = 2 \frac{(-1)^n}{n^2}$
	$(*) = \frac{1}{\pi} (2 \frac{(-1)^n}{n^2} + \frac{1}{n^2} - \frac{(-1)^n}{n^2}) = \frac{1}{\pi} (\frac{2 (-1)^n - (-1)^n + 1}{n^2}) = \frac{3(-1)^n - 1}{\pi n^2}$
- $b_n = \frac{1}{\pi} (\int\limits_{0}^{\pi} \frac{x^2}{\pi} \sin (nx) - \int\limits_{- \pi}^{0} x \sin (nx) dx) = (*)$
	$II = \begin{vmatrix} u = x \\ du = dx \\ dv = \sin (nx) dx \\ v = - \frac{\cos (nx)}{n} \end{vmatrix} = - x \frac{\cos (nx)}{n}|_{- \pi}^{0} + \int\limits_{- \pi}^{0} \frac{\cos (nx)}{n} dx = \pi \frac{\cos (\pi n)}{n} = \frac{\pi (-1)^n}{n}$
	$I = \begin{vmatrix} u = \frac{x^2}{\pi} \\ du = \frac{2x}{\pi}dx \\ dv = \sin (nx) dx \\ v = - \frac{\cos (nx)}{n} \end{vmatrix} = - \frac{x^2}{\pi} \cdot \frac{\cos (nx)}{n}|_{0}^{\pi} + \frac{2}{\pi} \int\limits_{0}^{\pi} x \frac{\cos (nx)}{n} dx = \begin{vmatrix} u = x \\ du = dx \\ dv = \frac{\cos (nx)}{n} dx \\ v = \frac{\sin (nx)}{n^2} \end{vmatrix} = \frac{-\pi \cdot (-1)^n}{n} + \frac{2}{\pi}(0 - \int\limits_{0}^{\pi} \frac{\sin (nx)}{n^2} dx) = \frac{- \pi (-1)^n}{n} + \frac{2}{\pi} (\frac{(-1)^n}{n^3} - \frac{1}{n^3})$
	$(*) = \frac{1}{\pi} (\frac{- \pi (-1)^n}{n} + \frac{2}{\pi}(\frac{(-1)^n}{n^3} - \frac{1}{n^3}) + \frac{\pi (-1)^n}{n}) = \frac{2}{\pi n^3} \cdot ((-1)^n - 1)$
- $f(x) =^{пв} = \frac{5 \pi}{12} + \sum\limits_{n = 1}^{\infty} (\frac{3(-1)^n - 1}{ n^2} \cos (nx) + \frac{1}{\pi^2 n^3} ((-1)^n - 1) \sin(nx))$

## Номер 2
Ряд Фурье в комплексную и вещественную форму:
$f(x) = \frac{1 - a^2}{1 - 2 a \cos(x) + a^2}, \ \text{где} \ |a| < 1, \ a \in \mathbb{R}$

$a_n = \frac{2}{n} \int\limits_{0}^{\pi} f(x) \cos(nx) dx = \frac{2 (1 - a^2)}{\pi} \int\limits_{0}^{\pi} \frac{\cos (nx) dx}{1 - 2 a \cos (x) + a^2}$

ДОМА

## Номер 3
$f(x) = x^2, \ x \in [-4; 4], \ S(x) = \sum\limits_{n = - \infty}^{\infty} C_n e^{inwx}$
$C_n = \frac{a_n - ib_n}{2} \implies \begin{cases} a_n = Re(2C_n) \\ b_n = - Im (2Cn) \end{cases}$
$T = 2 \cdot 4 = 8 \implies l = 4$
$C_n = \frac{1}{4} \int\limits_{-4}^{4} x^2 e^{-\frac{in \pi x}{4}}dx = \begin{vmatrix} u = x^2 \\ du = 2x dx \\ dv = e^{-\frac{in \pi x}{4}} dx \\ v = \frac-{4}{i \pi n} e^{- \frac{i \pi n x}{4}} \end{vmatrix} = \frac{1}{4}(x^2 \cdot (- \frac{4}{i \pi n}) e^{- \frac{i \pi n x}{4}}|_{-4}^{4}) = -\frac{1}{4} \int\limits_{-4}^{4} - \frac{4}{i \pi n} \cdot e^{- \frac{i \pi n x}{4}} \cdot 2 x dx = - \frac{1}{i \pi n} (4^2 \cdot e^{- i \pi n} - 4^2 \cdot e^{i \pi n}) + \frac{2}{i \pi n} \int\limits x \cdot e^{- \frac{i \pi n x}{4}} dx = \frac{64}{n^2 \pi^2} (-1)^n$
$C_0 = \frac{1}{4} \int\limits_{-4}^{4} x^2 e^0 dx = \frac{1}{4} \frac{x^3}{3}|_{-4}^{4} = \frac{1}{12} (4^3 + 4^3) = \frac{4^3}{6} = \frac{64}{6} = \frac{32}{3}$

$f(x) =^{пв} \frac{16}{3} + \frac{32}{\pi^2} + (\sum\limits_{- \infty}^{-1} \frac{(-1)^n}{n^2} e^{i n \frac{\pi}{4} x} + \sum\limits_{1}^{\infty} \frac{(-1)^n}{n^2} e^{i n \frac{\pi}{4}x})$