#матан 
$$F'_t = f'_x \cdot x'_t + f'_y \cdot y'_t$$
$$(F'_t)'_t = (f'_x \cdot x'_t + f'_y y'_t)'_t = (f'_x \cdot x'_t)'_t + (f'_y \cdot y'_t)'_t =$$
$$= (f'_x)'_t \cdot x'_t + f'_x \cdot (x'_t)'_t + (f'_y)'_t \cdot y'_t + f'_y \cdot (y'_t)'_t =$$
$$(f''_{xx} \cdot x'_t + f''_{xy} \cdot y'_t) \cdot x'_t + f'_x \cdot x''_{tt} + (f''_{yx} \cdot x'_t + f''_{yy} \cdot y'_t) \cdot y'_t + f'_y \cdot y''_{tt} =$$
$$= f''_{xx} (x'_t)^2 + 2 f''_{xy} \cdot y'_t \cdot x'_t + f''_{yy}(y'_t)^2 + f'_x \cdot x''_{tt} + f'_y \cdot y''_{tt}$$
Кринж какой-то, но юзабельно