#матан 
## Задание 1
$\lim\limits_{\alpha \to 0} \int\limits_{-1}^{1} \sqrt{x^2 + \alpha^2}dx = \int\limits_{-1}^{1} \lim\limits_{\alpha \to 0} \sqrt{x^2 + \alpha^2}dx = \int\limits_{-1}^{1} |x| dx = - \int\limits_{-1}^{0} x dx + \int\limits_{0}^{1} x dx = - \frac{x^2}{2}|_{-1}^{0} + \frac{x^2}{2}|_{0}^{1} = 0 + \frac{1}{2} + \frac{1}{2} + 0 = 1$

## Задание 2
$\lim\limits_{n \to \infty} \int\limits_{0}^{1} \frac{dx}{1 + (1 + \frac{x}{n})^n} = \int\limits_{0}^{1}\lim\limits_{n \to \infty} \frac{dx}{1 + (1 + \frac{x}{n})^n} = \int\limits_{0}^{1} \frac{dx}{1 + e^x} = \begin{vmatrix}t = 1 + e^x \\e^x = t - 1 \\x = \ln(t - 1) \\ dx = \frac{1}{t - 1} dt \end{vmatrix} = \int\limits_{2}^{1 + e} \frac{dt}{(t - 1)t} =$
$= \int\limits_{2}^{1 + e} \frac{A}{t - 1} dt + \int\limits_{2}^{1 + e} \frac{B}{t} dt = \int\limits_{2}^{1 + e} \frac{1}{t - 1} dt - \int\limits_{2}^{1 + e} \frac{1}{t} dt = \ln|t - 1||_{2}^{1 + e} - \ln(t) |_{2}^{1 + e} =$
$= \ln(e) - \ln(1) - (\ln(1 + e) - \ln(2)) = 1 - 0 - \ln(1 + e) + \ln(2) = 1 - \ln(1 + e) + \ln(2)$

## Задание 3
$\lim\limits_{\alpha \to \infty} \int\limits_{1}^{2} \frac{\ln(x + |\alpha|)}{\ln(x^2 + \alpha^2)} dx = \int\limits_{1}^{2} \lim\limits_{\alpha \to \infty} \frac{\ln(x + |\alpha|)}{\ln(x^2 + \alpha^2)} dx = \int\limits_{1}^{2} \lim\limits_{\alpha \to \infty} \frac{x^2 + \alpha^2}{x + |\alpha|} dx = \int\limits_{1}^{2} \frac{1}{2} dx = \frac{1}{2} \cdot 2 - \frac{1}{2} = \frac{1}{2}$

## Задание 4
$\lim\limits_{y \to 0} \int\limits_{0}^{1} \frac{x \cdot e^{- \frac{x^2}{y^2}}}{y^2} dx = \lim\limits_{y \to 0} \frac{1}{y^2} \int\limits_{0}^{1} x \cdot e^{- \frac{x^2}{y^2}} dx = \lim\limits_{y \to 0} \frac{1}{2} \int\limits_{0}^{1} e^{- \frac{x^2}{y^2}} (d \frac{x^2}{y^2}) = \lim\limits_{y \to 0} (-e^{- \frac{1}{y^2}}(\frac{1}{2}) + \frac{1}{2}) = \frac{1}{2}$

## Задание 5
$$\int\limits_{0}^{1} x^m \cdot \ln^n(x) dx$$
1) $\int\limits_{0}^{1} x^m dx = \frac{x^{m + 1}}{m + 1}|_{0}^{1} = \frac{1}{m + 1}$
2) $\frac{d(\int\limits_{0}^{1} x^m dx)}{dm} = \int\limits_{0}^{1} (x^m)'_m dx = \int\limits_{0}^{1} x^m \ln(x) dx = \begin{vmatrix}u =\ln(x) \\dv = x^m dx \\du = \frac{dx}{x} \\v = \frac{x^{m + 1}}{m + 1}\end{vmatrix} = (\ln x \cdot \frac{x^{m + 1}}{m + 1})|_{0}^{1} - \frac{1}{m - 1} \int\limits_{0}^{1} x^m dx = - \frac{1}{(m + 1)^2}$

$\int\limits_{0}^{1} x^m \cdot \ln^n(x) dx = \frac{d(- \frac{1}{(m + 1)^2})}{dm} = (-(m + 1)^2)'_m = 2! \cdot \frac{1}{(m + 1)^3} \implies (-1)^n \frac{n!}{(m + 1)^{n + 1}}$

## Задание 6
$\lim\limits_{y \to 0} \int\limits_{y}^{1 + y} \sqrt{x^2 + y^2} dx = \int\limits_{0}^{1} |x| dx = 1$

$\lim\limits_{y \to 0} \int\limits_{1 + y}^{2 + y^2} \frac{dx}{1 + x^2 + y^2} = arctg (2) - arctg(1) = arctg(2) - \frac{\pi}{4}$

$\frac{d(\int\limits_{y}^{1 + y} \sqrt{x^2 + y^2} dx)}{dy} = \int\limits_{y}^{1 + y} (\sqrt{x^2 + y^2})'_y dx + 1 \sqrt{(1 + y)^2 + y^2} - \sqrt{2y^2} = \int\limits_{y}^{1 + y} \frac{dx}{2 \sqrt{x^2 + y^2}}2y + \dots = y \cdot \ln|1 + \sqrt{x^2 + y^2}|$