#матан 
## Задание 1
$\lim\limits_{y \to 0}\int\limits_{0}^{1} \frac{dx}{1 + x^2 + y^2} = \int\limits_{0}^{1} \lim\limits_{y \to 0} \frac{1}{1 + x^2 + y^2}dx = \int\limits_{0}^{1} \frac{1}{1 + x^2} dx = arctg \ x|_{0}^{1} = arctg \ 1 - arctg \ 0 = \frac{\pi}{4}$

## Задание 2
$\lim\limits_{y \to 0}\int\limits_{-1}^{1} \sqrt{x^2 + y^2}dx = \int\limits_{-1}^{1} \lim\limits_{y \to 0} \sqrt{x^2 + y^2}dx = \int\limits_{-1}^{1} |x|dx = - \int\limits_{-1}^{0} xdx + \int\limits_{0}^{1} xdx = -(\frac{x^2}{2}|_{-1}^{0}) + (\frac{x^2}{2}|_{0}^{1}) = \frac{1}{2} + \frac{1}{2} = 1$

## Задание 3
$\lim\limits_{y \to 0}\int\limits_{y}^{1 + y} \frac{dx}{1 + x^2 + y^2} = \int\limits_{y}^{y + 1}\lim\limits_{y \to 0} \frac{1}{1 + x^2 + y^2} dx = \int\limits_{0}^{1} \frac{dx}{1 + x^2} = \frac{\pi}{4}$ - то же самое, что и в первом

## Задание 4
$J(y) = \int\limits_{0}^{1} \frac{xdx}{1 + x^2 + y^2}$
$\frac{J(y)}{dy} = \int\limits_{0}^{1} \frac{-2 y x dx}{(1 + x^2 + y^2)^2} = -y \int\limits_{0}^{1} \frac{2xdx}{(1 + x^2 + y^2)^2} = -y \int\limits_{y^2 + 1}^{y^2 + 2} \frac{d(x^2 + y^2 + 1)}{(1 + x^2 + y^2)^2} = -y \cdot (-1) \cdot (1 + x^2 + y^2)^{-1}|_{y^2 + 1}^{y^2 + 2} = y((y^2 + 2)^{-1} - (y^2 + 1)^{-1}) = \frac{y}{y^2 + 2} - \frac{y}{y^2 + 1} = y \cdot \frac{y^2 + 1 - y^2 - 2}{(y^2 + 2)(y^2 + 1)} = y \cdot \frac{-y}{(y^2 + 2)(y^2 + 1)}$

## Задание 5
$I(\alpha) = \int\limits_{0}^{\alpha} \frac{\ln(1 + \alpha x)}{1 + x^2} dx$
$I'(\alpha) = \int\limits_{0}^{\alpha} (\frac{\ln(1 + \alpha x)}{1 + x^2})'_{\alpha} dx + \frac{\ln(1 + \alpha x)}{(1 + x^2)}|_{x = \alpha} \frac{d\alpha}{d\alpha} = \int\limits_{0}^{\alpha} x \cdot \frac{1}{1 + \alpha x} \cdot \frac{1}{1 + x^2} dx + \frac{\ln(1 + \alpha ^2)}{(1 + \alpha^2)} = \int\limits_{0}^{\alpha} \frac{xdx}{1 + \alpha x + x^2 + dx^3} =$

С помощью метода неопределённых коэффициентов решаем дробь, получаем:
$\begin{cases} A + C = 0 \\ A + \alpha B = 0 \\ B + \alpha C = 1 \end{cases}$

$\begin{cases} B = \frac{1}{1 + \alpha^2} \\ C = \frac{\alpha}{1 + \alpha^2} \\ A = \frac{- \alpha}{1 + \alpha^2} \end{cases}$

$= \int\limits_{0}^{\alpha} \frac{\frac{- \alpha}{1 + \alpha^2}}{1 + \alpha x}dx + \int\limits_{0}^{\alpha} \frac{\frac{x + \alpha}{1 + \alpha^2}}{1 + \alpha x}dx + \int\limits_{0}^{\alpha} \frac{\ln(1 + \alpha^2)}{1 + \alpha x}dx = - \alpha \int\limits_{0}^{\alpha} \frac{dx}{(1 + \alpha^2)(1 + \alpha x)} + \frac{1}{1 + \alpha^2} \int\limits_{0}^{\alpha} \frac{x + \alpha}{(1 + x^2)}dx + \frac{\ln(1 + \alpha^2)}{1 + \alpha^2} =$
$= - \frac{1}{1 + \alpha^2} \cdot \ln(1 + \alpha x) + \frac{1}{2(1 + \alpha^2)} \int\limits_{0}^{\alpha} \frac{1}{(1 + x^2)}dx + \frac{\alpha}{(1 + \alpha^2)} \int\limits_{0}^{\alpha} \frac{\alpha x}{(1 + x^2)} + \frac{\ln(1 + \alpha^2)}{1 + \alpha^2} dx =$
$= \frac{- \ln(1 + \alpha x)}{1 + \alpha^2}|_{0}^{\alpha} + \frac{\ln(1 + \alpha^2)}{1 + \alpha^2} + \frac{1}{2(1 + \alpha^2)} \ln(1 + x^2)|_{0}^{\alpha} + \frac{\alpha}{1 + \alpha^2} \cdot arctg \ x|_{0}^{\alpha} = \frac{- \ln(1 + \alpha^2)}{1 + \alpha^2} + \frac{\ln(1 + \alpha^2)}{1 + \alpha^2} + \frac{\ln(1 + \alpha^2)}{2(1 + \alpha^2)} + \frac{\alpha \cdot arctg(\alpha)}{(1 + \alpha^2)}$

## Задание 6
$I(\alpha) = \int\limits_{1}^{2} e^{\alpha x^2} \frac{dx}{x}$
$I'_{\alpha}(\alpha) = \int\limits_{1}^{2} \frac{1}{x} e^{\alpha x^2} \cdot x^2 dx = \int\limits_{1}^{2} x e^{\alpha x} dx = \frac{1}{2} \int\limits_{1}^{2} e^{\alpha x} dx^2 = \frac{1}{2 \alpha} \int\limits_{1}^{2} e^{\alpha x^2} d(\alpha x^2) = \frac{1}{2 \alpha} (e^{4 \alpha} - e^{\alpha}) = \frac{e^{4 \alpha} - e^{\alpha}}{2\alpha}$