#тч 
1. Возьмём $a \neq 0, \ b \neq 0$
2. $b = q_0 \cdot a + r_0, \ N(r_0) < N(a)$
3. $a = q_1 \cdot r_0 + r_1, \ N(r_1) < N(r_0)$
4. $r_0 = q_2 \cdot r_1 + r_2, \ N(r_2) < N(r_1)$
5. $\dots$
6. $N(a) > N(r_0) > N(r_1) > \dots \implies r_{n + 1} = 0$
В какой-то момент дойдём до равенства $r_{n - 1} = q_n \cdot r_n + r_{n + 1}$, где $r_{n + 1} = 0$, тогда $r_n$ - НОД(a, b).

По [[Свойства НОД|6-ому свойству НОД]]: НОД(a, b) = НОД(a, r), так как $b = aq + r$.
По [[Свойства НОД|3-ему свойству НОД]]: НОД(a, 0) = a

Тогда: НОД(a, b) = НОД(a, $r_0$) = НОД($r_0, \ r_1$) = $\dots$ = НОД($r_n, \ r_{n + 1}$) = $r_n$